CLean.lean
@@ -4,4 +4,5 @@ import CLean.State
 import CLean.Typing
 import CLean.Helpers
 import CLean.Semantics
+import CLean.Lemmas
 import CLean.Examples
